specs/Spec.HSalsa20.fst
@@ -8,8 +8,8 @@ open FStar.UInt32
 open FStar.Endianness
 open Seq.Create
 open Spec.Lib
-
-module Salsa20 = Spec.Salsa20
+open Spec.Salsa20
+//module Salsa20 = Spec.Salsa20
 
 let keylen = 32 (* in bytes *)
 let blocklen = 64  (* in bytes *)
@@ -30,11 +30,39 @@ let setup (k:key) (n:nonce): state =
   let k_snd_half = slice ks 4 8 in
   create_16 Salsa20.constant0 (index ks 0)      (index ks 1)      (index ks 2)
           (index ks 3)       Salsa20.constant1 (index ns 0)      (index ns 1)
-	  (index ns 2)       (index ns 3)      Salsa20.constant2 (index ks 4)
+    (index ns 2)       (index ns 3)      Salsa20.constant2 (index ks 4)
           (index ks 5)       (index ks 6)      (index ks 7)      Salsa20.constant3
 
-let hsalsa20 (k:key) (n:nonce) : Tot key = 
+let hsalsa20 (k:key) (n:nonce) : Tot key =
   let st = setup k n in
   let st' = Spec.Salsa20.rounds st in
   let hs = create_8 st'.[0] st'.[5] st'.[10] st'.[15] st'.[6] st'.[7] st'.[8] st'.[9] in
   uint32s_to_le 8 hs
+
+
+unfold let k = [
+       0x4auy;0x5duy;0x9duy;0x5buy;0xa4uy;0xceuy;0x2duy;0xe1uy;
+       0x72uy;0x8euy;0x3buy;0xf4uy;0x80uy;0x35uy;0x0fuy;0x25uy;
+       0xe0uy;0x7euy;0x21uy;0xc9uy;0x47uy;0xd1uy;0x9euy;0x33uy;
+       0x76uy;0xf0uy;0x9buy;0x3cuy;0x1euy;0x16uy;0x17uy;0x42uy]
+
+unfold let zero = [
+       0x00uy;0x00uy;0x00uy;0x00uy;0x00uy;0x00uy;0x00uy;0x00uy;
+       0x00uy;0x00uy;0x00uy;0x00uy;0x00uy;0x00uy;0x00uy;0x00uy]
+
+unfold let k1 = [
+       0x1buy;0x27uy;0x55uy;0x64uy;0x73uy;0xe9uy;0x85uy;0xd4uy;
+       0x62uy;0xcduy;0x51uy;0x19uy;0x7auy;0x9auy;0x46uy;0xc7uy;
+       0x60uy;0x09uy;0x54uy;0x9euy;0xacuy;0x64uy;0x74uy;0xf2uy;
+       0x06uy;0xc4uy;0xeeuy;0x08uy;0x44uy;0xf6uy;0x83uy;0x89uy]
+
+
+let test() =
+    assert_norm(List.Tot.length k = 32);
+    assert_norm(List.Tot.length zero = 16);
+    assert_norm(List.Tot.length k1 = 32);
+    let k = createL k in
+    let zero = createL zero in
+    let k1 = createL k1 in
+    let k1' = hsalsa20 k zero in
+    k1 = k1'
